src/Math/NatArith.dfy
@@ -1,0 +1,11 @@
+module NatArith {
+  function Max(a: nat, b: nat): nat {
+    if a < b then b else a
+  }
+
+  function Min(a: nat, b: nat): nat {
+    if a < b then a else b
+  }
+
+  // TODO: a lot of functions from the helper module should go here.
+}
